Show Proof of concept for range iter

BPlusTree_ImpRange.thy
@@ -41,10 +41,10 @@ locale imp_split2 = abs_split_range: split_range split lrange_list + imp_split_r
   <pfa_is_it c ks (a',n') (lrange_list x ks)>\<^sub>t"
 begin
 
-partial_function (heap) lrange_iter_init ::
+partial_function (heap) leafs_range ::
   "'a btnode ref \<Rightarrow> 'a \<Rightarrow> 'a btnode ref option Heap"
   where
-    "lrange_iter_init p x = do {
+    "leafs_range p x = do {
   node \<leftarrow> !p;
   (case node of
      Btleaf xs z \<Rightarrow> do {
@@ -57,18 +57,18 @@ partial_function (heap) lrange_iter_init ::
        if i < tsl then do {
          s \<leftarrow> pfa_get ts i;
          let (sub,sep) = s in
-           lrange_iter_init (the sub) x
+           leafs_range (the sub) x
        } else
-           lrange_iter_init t x
+           leafs_range t x
     }
 )}"
 
 
 (* HT when expressed on list of leaves 
-lemma lrange_iter_init_rule:
+lemma leafs_range_rule:
   assumes "k > 0" "root_order k t"
   shows "<bplustree_assn_leafs k t ti r z lptrs>
-lrange_iter_init ti x
+leafs_range ti x
 <\<lambda>p. (\<exists>\<^sub>A xs1 xs2 lptrs1 lptrs2 ps.
   inner_nodes_assn k t ti r z lptrs *
   leaf_nodes_assn k xs1 r p lptrs1 *
@@ -83,10 +83,10 @@ sorry
 *)
 
 (* much shorter when expressed on the nodes themselves *)
-lemma lrange_iter_init_rule:
+lemma leafs_range_rule:
   assumes "k > 0" "root_order k t"
   shows "<bplustree_assn_leafs k t ti r z lptrs>
-lrange_iter_init ti x
+leafs_range ti x
 <\<lambda>p. (\<exists>\<^sub>A xs1 lptrs1 lptrs2.
   inner_nodes_assn k t ti r z lptrs *
   leaf_nodes_assn k xs1 r p lptrs1 *
@@ -97,15 +97,175 @@ lrange_iter_init ti x
 >\<^sub>t"
   apply(induction t x rule: abs_split_range.leafs_range.induct)
   subgoal for ks x
-    apply(subst lrange_iter_init.simps)
+    apply(subst leafs_range.simps)
     apply (sep_auto eintros del: exI)
     apply(inst_existentials "[]::'a bplustree list" "[]::'a btnode ref list" "[ti]")
     apply sep_auto+
     done
   subgoal for ts t x
-    apply(subst lrange_iter_init.simps)
-    apply (sep_auto heap add: imp_split_rule)
+    apply(subst leafs_range.simps)
+    (*apply (sep_auto heap add: imp_split_rule)*)
+    sorry
+  done
   (* TODO *)
+
+(*fun concat_leafs_range where
+  "concat_leafs_range t x = (case leafs_range t x of (LNode ks)#list \<Rightarrow> lrange_list x ks @ (concat (map leaves list)))"
+*)
+
+definition concat_leafs_range where
+"concat_leafs_range ti x = do {
+  lp \<leftarrow> leafs_range ti x;
+  li \<leftarrow> !(the lp);
+  case li of Btleaf xs nxt \<Rightarrow> do {
+    arr_it \<leftarrow> imp_lrange_list x xs;
+    fla_it \<leftarrow> leaf_elements_adjust (nxt,None) arr_it;
+    return fla_it
+  }
+}"
+
+lemma sorted_less_leaf_nodes: "sorted_less (leaves t) \<Longrightarrow> (LNode ks) \<in> set (leaf_nodes t) \<Longrightarrow> sorted_less ks"
+proof(induction t arbitrary: ks rule: leaf_nodes.induct)
+  case (1 xs)
+  then show ?case by simp
+next
+  case I: (2 ts t)
+  then have "(\<exists>x \<in> set ts. LNode ks \<in> set (leaf_nodes (fst x))) \<or> LNode ks \<in> set (leaf_nodes t)"
+    by simp
+  then show ?case 
+  proof(standard, goal_cases)
+    case 1
+    then show ?case
+      using I
+      by (metis (no_types, lifting) in_set_conv_decomp list.simps(9) map_append sorted_leaves_subtrees)
+  next
+    case 2
+    then show ?case
+      using I
+      by (meson sorted_leaves_induct_last)
+  qed
+qed
+
+lemmas leaf_elements_adjust_rule = leaf_elements_iter.flatten_it_adjust_rule
+
+lemma leaf_elements_adjust_rule_tweaked:
+"<list_assn (is_pfa (2 * k)) ls1' ls1 * list_assn (is_pfa (2 * k)) ls2' ls2 *
+     leaf_iter_assn (ls1 @ lsim # ls2) lptrs lsi ls2 oit *
+     pfa_is_it (2 * k) (lsm1 @ lsm2) lsim lsm2 iit *
+    list_assn leaf_node (leaf_nodes t) (leaf_lists t) *
+    inner_nodes_assn k t ti r None lptrs * true
+>
+  leaf_elements_adjust oit iit
+<\<lambda>it. leaf_elements_iter.is_flatten_it lptrs k (ls1' @ (lsm1 @ lsm2) # ls2') (concat (ls1' @ (lsm1 @ lsm2) # ls2')) lsi (concat (lsm2 # ls2')) it *
+    list_assn leaf_node (leaf_nodes t) (leaf_lists t) *
+    inner_nodes_assn k t ti r None lptrs
+>\<^sub>t"
+  by (sep_auto heap: leaf_elements_adjust_rule)
+
+lemma concat_leafs_range_rule:
+  assumes "k > 0" "root_order k t" "sorted_less (leaves t)"
+  shows "<bplustree_assn_leafs k t ti r None lptrs>
+concat_leafs_range ti x
+<leaf_elements_iter k t ti r (abs_split_range.lrange t x)>\<^sub>t"
+  apply(subst concat_leafs_range_def)
+  apply(vcg (ss) heap: leafs_range_rule)+
+  subgoal using assms by simp
+  subgoal using assms by simp
+  apply simp
+  apply(rule norm_pre_ex_rule)+
+  apply(rule hoare_triple_preI)
+  apply(auto dest!: mod_starD)
+proof(goal_cases)
+  case (1 l xs1 lptrs1 lptrs2)
+  obtain ks list where [simp]: "abs_split_range.leafs_range t x = (LNode ks)#list \<and> (LNode ks) \<in> set (leaf_nodes t)"
+    using abs_split_range.leafs_range_not_empty by blast
+  then obtain r' lptrs2' where [simp]: "lptrs2 = r' # lptrs2'"
+    using 1
+    by (metis Suc_length_conv leaf_nodes_assn_impl_length)
+  have sorted_less_ks: "sorted_less ks"
+    using \<open>abs_split_range.leafs_range t x = LNode ks # list \<and> LNode ks \<in> set (leaf_nodes t)\<close> assms(3) imp_split2.sorted_less_leaf_nodes imp_split2_axioms by blast
+  then obtain pref where ks_split: "ks = pref @ lrange_list x ks"
+  proof (goal_cases)
+    case 1
+    have "suffix (lrange_list x ks) ks"
+      by (metis \<open>sorted_less ks\<close> abs_split_range.lrange_list_req lrange_suffix sorted_less_lrange)
+    then have "\<exists>pref. ks = pref @ lrange_list x ks"
+      by (meson suffixE)
+    then show ?case
+      using 1
+      by blast
+  qed
+  show ?case
+  proof(cases l)
+    case None
+    show ?thesis
+      apply(rule hoare_triple_preI)
+      using None by simp
+  next
+  case (Some a)
+    then show ?thesis
+      apply simp
+      apply(rule norm_pre_ex_rule)+
+      apply vcg
+      apply simp
+      subgoal for xsi fwd
+        apply(cases xsi)
+        apply simp
+      thm lrange_list_rule
+      using sorted_less_ks apply (vcg  heap: lrange_list_rule)
+      apply(subst leaf_nodes_assn_flatten)+
+      apply(simp)
+      apply(rule norm_pre_ex_rule)+
+      subgoal for ksia ksin it ps2 ps1
+      supply R = Hoare_Triple.cons_pre_rule[rotated, OF leaf_elements_adjust_rule_tweaked]
+        thm R
+        supply R' = R[of _ k "map leaves xs1" ps1 "map leaves list" ps2 "(ksia,ksin)"
+                         "lptrs1 @ r' # lptrs2'" r "(fwd,None)" pref "lrange_list x ks"
+                         it t ti r]
+      thm R'
+      apply(vcg heap: R')
+      thm leaf_iter_assn_def
+      apply(subst leaf_iter_assn_def)
+      apply simp
+      subgoal
+        apply(inst_ex_assn "ps1@[(ksia,ksin)]" "lptrs1@[r']" lptrs2')
+        apply sep_auto
+          subgoal
+            apply(rule entails_preI)
+            apply(subst leafs_assn_aux_append)
+            subgoal by (auto dest!: mod_starD leafs_assn_impl_length)
+            subgoal
+              apply simp
+              apply(inst_ex_assn "Some r'")
+              apply(subgoal_tac "leaf_lists t = (map leaves xs1 @ ks # map leaves list)")
+              apply(subgoal_tac "pref @ lrange_list x ks = ks")
+              apply(subgoal_tac "leaf_nodes t = xs1 @ (LNode ks) # list")
+              subgoal by sep_auto
+              subgoal sorry
+              subgoal using ks_split by simp
+              subgoal sorry
+              done
+        done
+      done
+      subgoal
+        apply (sep_auto eintros del: exI simp add: leaf_elements_iter_def)
+        apply(inst_existentials lptrs)
+        apply(subgoal_tac "lptrs = lptrs1 @ r' # lptrs2'")
+        apply(subgoal_tac "leaf_lists t = (map leaves xs1 @ (pref @ lrange_list x ks) # map leaves list)")
+        apply(subgoal_tac "leaves t = (concat (map leaves xs1) @ pref @ lrange_list x ks @ concat (map leaves list))")
+        apply(subgoal_tac "abs_split_range.lrange t x = (lrange_list x ks @ concat (map leaves list))")
+        subgoal by sep_auto
+        subgoal by (metis \<open>abs_split_range.leafs_range t x = LNode ks # list \<and> LNode ks \<in> set (leaf_nodes t)\<close> abs_split_range.split_range_axioms split_range.leafs_range_pre_lrange)
+        subgoal sorry
+        subgoal sorry
+        subgoal sorry
+        done
+      done
+    done
+  done
+  qed
+qed
+
 
 end
 
